f.v
@@ -41,14 +41,21 @@ Module exprop.
   Defined.
 End exprop.
 
-Module type.
-  Module A := abt.internal tyop.
+Module type_abt := abt.abt tyop.
 
+Module type_ast.
   Inductive t :=
   | var (alpha : nat) : t
   | arrow : t -> t -> t
   | all : t -> t
   .
+End type_ast.
+
+Module type_basis.
+  Module A := type_abt.
+
+  Import type_ast.
+  Definition t := t.
 
   Fixpoint to_abt (ty : t) : A.t :=
     match ty with
@@ -94,8 +101,8 @@ Module type.
     | all ty' => all (shift (S c) d ty')
     end.
 
-  Lemma shift_to_of_abt : forall ty c d, shift c d ty = of_abt (A.shift c d (to_abt ty)).
-  Proof. induction ty; simpl; intros c d; f_equal; auto. Qed.
+  Lemma shift_to_abt_comm : forall ty c d, to_abt (shift c d ty) = A.shift c d (to_abt ty).
+  Proof. induction ty; simpl; intros c d; auto; repeat f_equal; auto. Qed.
     
   Fixpoint subst rho ty :=
     match ty with
@@ -107,11 +114,6 @@ Module type.
     | all ty' => all (subst (var 0 :: map (shift 0 1) rho) ty')
     end.
 
-  Hint Resolve A.ws_shift ws_to_abt.
-
-  Lemma shift_to_abt_comm : forall ty c d, to_abt (shift c d ty) = A.shift c d (to_abt ty).
-  Proof. intros. rewrite shift_to_of_abt, to_of_abt; auto. Qed.
-
   Lemma map_shift_to_abt_comm :
     forall c d rho, map to_abt (map (shift c d) rho) = map (A.shift c d) (map to_abt rho).
   Proof.
@@ -119,15 +121,13 @@ Module type.
     rewrite !map_map.
     now erewrite map_ext by (intros; apply shift_to_abt_comm).
   Qed.
-  
-  Lemma subst_to_of_abt :
-    forall ty rho,
-      subst rho ty = of_abt (A.subst (map to_abt rho) (to_abt ty)).
+
+  Lemma subst_to_abt_comm : forall ty rho,
+      to_abt (subst rho ty) = A.subst (map to_abt rho) (to_abt ty).
   Proof.
-    induction ty; simpl; intros rho; try rewrite ?A.descend_0, ?A.descend_1; f_equal; auto.
-    - rewrite nth_error_map.
-      break_match; auto.
-      now rewrite of_to_abt.
+    unfold t.
+    induction ty; simpl; intros rho; rewrite ?A.descend_0, ?A.descend_1; repeat f_equal; auto.
+    - rewrite nth_error_map. break_match; auto.
     - rewrite IHty. simpl.
       now rewrite map_shift_to_abt_comm.
   Qed.
@@ -142,207 +142,31 @@ Module type.
   Lemma wf_to_abt : forall ty n, wf n ty <-> A.wf n (to_abt ty).
   Proof. induction ty; simpl; firstorder. Qed.
 
-  Lemma wf_of_abt :
-    forall a n,
-      A.ws a -> 
-      wf n (of_abt a) <-> A.wf n a.
-  Proof.
-    intros.
-    pose proof wf_to_abt (of_abt a) n.
-    rewrite to_of_abt in *; auto.
-  Qed.
-
   Fixpoint identity_subst (n : nat) : list t :=
     match n with
     | 0 => []
     | S n => var 0 :: map (shift 0 1) (identity_subst n)
     end.
 
-  Lemma shift_of_abt_comm :
-    forall a c d,
-      A.ws a -> 
-      shift c d (of_abt a) = of_abt (A.shift c d a).
-  Proof.
-    intros a c d WS.
-    rewrite shift_to_of_abt.
-    now rewrite to_of_abt by assumption.
-  Qed.
-
-  Lemma map_shift_of_abt_comm :
-    forall rho c d,
-      Forall A.ws rho -> 
-      map (shift c d) (map of_abt rho) = map of_abt (map (A.shift c d) rho).
-  Proof.
-    intros rho c d WS.
-    rewrite !map_map.
-    apply map_ext_in.
-    intros a I.
-    rewrite shift_of_abt_comm; auto.
-    eapply Forall_forall; eauto.
-  Qed.
-
-  Lemma identity_subst_of_abt :
+  Lemma identity_subst_to_abt_comm :
     forall n,
-      identity_subst n = List.map of_abt (A.identity_subst n).
+      List.map to_abt (identity_subst n) = A.identity_subst n.
   Proof.
     induction n; simpl; f_equal; auto.
-    rewrite IHn.
-    rewrite map_shift_of_abt_comm; auto.
-    apply A.ws_identity_subst.
+    now rewrite map_shift_to_abt_comm, IHn.
   Qed.
+End type_basis.
 
-  Lemma wf_shift : forall ty c d n, wf n ty -> wf (d + n) (shift c d ty).
-  Proof.
-    intros.
-    rewrite shift_to_of_abt.
-    rewrite wf_of_abt; auto.
-    apply A.wf_shift.
-    now rewrite <- wf_to_abt.
-  Qed.
-
-  Lemma wf_subst : forall ty n rho, wf (length rho) ty -> Forall (wf n) rho -> wf n (subst rho ty).
-  Proof.
-    intros ty n rho WF F.
-    rewrite subst_to_of_abt.
-    rewrite wf_of_abt.
-    - apply A.wf_subst.
-      + now rewrite map_length, <- wf_to_abt.
-      + rewrite Forall_map.
-        eapply Forall_impl; try eassumption.
-        intros ty' WF'.
-        now rewrite <- wf_to_abt.
-    - apply A.ws_subst; auto.
-      rewrite Forall_map.
-      apply Forall_forall; auto.
-  Qed.
-
-  Lemma identity_subst_length : forall n, length (identity_subst n) = n.
-  Proof.
-    intros.
-    rewrite identity_subst_of_abt.
-    rewrite map_length.
-    apply A.identity_subst_length.
-  Qed.
-
-  Lemma wf_identity_subst: forall n : nat, Forall (wf n) (identity_subst n).
-  Proof.
-    intros.
-    rewrite identity_subst_of_abt.
-    rewrite Forall_map.
-    rewrite Forall_forall.
-    intros ty I.
-    rewrite wf_of_abt.
-    - eapply Forall_forall; [apply A.wf_identity_subst|]; auto.
-    - eapply Forall_forall; [apply A.ws_identity_subst|]; eauto.
-  Qed.
-
-  Lemma wf_weaken : forall ty n d, n <= d -> wf n ty -> wf d ty.
-  Proof.
-    intros ty n d LE.
-    rewrite !wf_to_abt.
-    eauto using A.wf_weaken.
-  Qed.
-
-  Lemma shift_merge : forall ty c d1 d2 , shift c d2 (shift c d1 ty) = shift c (d2 + d1) ty.
-  Proof.
-    intros ty c d1 d2.
-    rewrite !shift_to_of_abt.
-    rewrite to_of_abt by auto.
-    now rewrite A.shift_merge.
-  Qed.
-
-  Lemma shift_nop_d :
-    forall ty c,
-      shift c 0 ty = ty.
-  Proof.
-    intros ty c.
-    rewrite shift_to_of_abt.
-    rewrite A.shift_nop_d.
-    now rewrite of_to_abt.
-  Qed.
-
-  Lemma subst_to_abt_comm : forall ty rho, to_abt (subst rho ty) = A.subst (map to_abt rho) (to_abt ty).
-  Proof.
-    intros. rewrite subst_to_of_abt, to_of_abt; auto.
-    apply A.ws_subst; auto.
-    rewrite Forall_map.
-    apply Forall_forall.
-    auto.
-  Qed.
-
-  Lemma map_subst_to_abt_comm :
-    forall rho1 rho2,
-      map to_abt (map (subst rho2) rho1) =
-      map (A.subst (map to_abt rho2)) (map to_abt rho1).
-  Proof.
-    intros rho1 rho2.
-    rewrite !map_map.
-    apply map_ext.
-    intros ty'.
-    auto using subst_to_abt_comm.
-  Qed.
-
-  Lemma subst_subst :
-    forall ty rho1 rho2,
-      wf (List.length rho1) ty ->
-      List.Forall (wf (List.length rho2)) rho1 ->
-      subst rho2 (subst rho1 ty) =
-      subst (List.map (subst rho2) rho1) ty.
-  Proof.
-    intros ty rho1 rho2 WF F.
-    rewrite !subst_to_of_abt.
-    rewrite !to_of_abt.
-    - rewrite A.subst_subst.
-      + now rewrite map_subst_to_abt_comm.
-      + now rewrite map_length, <- wf_to_abt.
-      + rewrite map_length, Forall_map.
-        eapply Forall_impl; try eassumption.
-        intros ty'.
-        now rewrite wf_to_abt.
-    - apply A.ws_subst; auto.
-      rewrite Forall_map.
-      apply Forall_forall; auto.
-  Qed.
-
-  Lemma subst_shift_singleton :
-    forall ty ty',
-      wf 0 ty ->
-      subst [ty'] (shift 0 1 ty) = ty.
-  Proof.
-    intros.
-    rewrite subst_to_of_abt, shift_to_of_abt.
-    simpl.
-    rewrite to_of_abt.
-    - rewrite A.subst_shift_singleton.
-      + now rewrite of_to_abt.
-      + now rewrite <- wf_to_abt.
-    - apply A.ws_shift; auto.
-  Qed.
-
-  Lemma subst_identity :
-    forall ty n,
-      subst (identity_subst n) ty = ty.
-  Proof.
-    intros ty n.
-    rewrite subst_to_of_abt, identity_subst_of_abt.
-    rewrite !map_map.
-    erewrite map_ext_in.
-    rewrite map_id.
-    rewrite A.subst_identity.
-    now rewrite of_to_abt.
-    intros ty' I.
-    simpl.
-    rewrite to_of_abt; auto.
-    eapply Forall_forall.
-    apply A.ws_identity_subst.
-    eauto.
-  Qed.
-
+Module type.
+   Include abt.abt_util type_basis.
+   Notation var := type_ast.var.
+   Notation arrow := type_ast.arrow.
+   Notation all := type_ast.all.
 End type.
 
-Module expr.
-  Module A := abt.internal exprop.
+Module expr_abt := abt.abt exprop.
 
+Module expr_ast.
   Inductive t :=
   | var (x : nat) : t
   | abs : t -> t
@@ -350,6 +174,13 @@ Module expr.
   | tyabs : t -> t
   | tyapp : t -> t
   .
+End expr_ast.
+
+Module expr_basis.
+  Module A := expr_abt.
+
+  Import expr_ast.
+  Definition t := t.
 
   Fixpoint to_abt (ty : t) : A.t :=
     match ty with
@@ -401,9 +232,9 @@ Module expr.
     | tyapp e' => tyapp (shift c d e')
     end.
 
-  Lemma shift_to_of_abt : forall e c d, shift c d e = of_abt (A.shift c d (to_abt e)).
-  Proof. induction e; simpl; intros c d; f_equal; auto. Qed.
-    
+  Lemma shift_to_abt_comm : forall e c d, to_abt (shift c d e) = A.shift c d (to_abt e).
+  Proof. induction e; simpl; intros c d; auto; repeat f_equal; auto. Qed.
+
   Fixpoint subst rho e :=
     match e with
     | var x => match nth_error rho x with
@@ -416,11 +247,6 @@ Module expr.
     | tyapp e' => tyapp (subst rho e')
     end.
 
-  Hint Resolve A.ws_shift ws_to_abt.
-
-  Lemma shift_to_abt_comm : forall e c d, to_abt (shift c d e) = A.shift c d (to_abt e).
-  Proof. intros. rewrite shift_to_of_abt, to_of_abt; auto. Qed.
-
   Lemma map_shift_to_abt_comm :
     forall c d rho, map to_abt (map (shift c d) rho) = map (A.shift c d) (map to_abt rho).
   Proof.
@@ -428,15 +254,13 @@ Module expr.
     rewrite !map_map.
     now erewrite map_ext by (intros; apply shift_to_abt_comm).
   Qed.
-  
-  Lemma subst_to_of_abt :
-    forall e rho,
-      subst rho e = of_abt (A.subst (map to_abt rho) (to_abt e)).
+
+  Lemma subst_to_abt_comm : forall e rho,
+      to_abt (subst rho e) = A.subst (map to_abt rho) (to_abt e).
   Proof.
-    induction e; simpl; intros rho; try rewrite ?A.descend_0, ?A.descend_1; f_equal; auto.
-    - rewrite nth_error_map.
-      break_match; auto.
-      now rewrite of_to_abt.
+    unfold t.
+    induction e; simpl; intros rho; rewrite ?A.descend_0, ?A.descend_1; repeat f_equal; auto.
+    - rewrite nth_error_map. break_match; auto.
     - rewrite IHe. simpl.
       now rewrite map_shift_to_abt_comm.
   Qed.
@@ -453,201 +277,28 @@ Module expr.
   Lemma wf_to_abt : forall e n, wf n e <-> A.wf n (to_abt e).
   Proof. induction e; simpl; firstorder. Qed.
 
-  Lemma wf_of_abt :
-    forall a n,
-      A.ws a -> 
-      wf n (of_abt a) <-> A.wf n a.
-  Proof.
-    intros.
-    pose proof wf_to_abt (of_abt a) n.
-    rewrite to_of_abt in *; auto.
-  Qed.
-
   Fixpoint identity_subst (n : nat) : list t :=
     match n with
     | 0 => []
     | S n => var 0 :: map (shift 0 1) (identity_subst n)
     end.
 
-  Lemma shift_of_abt_comm :
-    forall a c d,
-      A.ws a -> 
-      shift c d (of_abt a) = of_abt (A.shift c d a).
-  Proof.
-    intros a c d WS.
-    rewrite shift_to_of_abt.
-    now rewrite to_of_abt by assumption.
-  Qed.
-
-  Lemma map_shift_of_abt_comm :
-    forall rho c d,
-      Forall A.ws rho -> 
-      map (shift c d) (map of_abt rho) = map of_abt (map (A.shift c d) rho).
-  Proof.
-    intros rho c d WS.
-    rewrite !map_map.
-    apply map_ext_in.
-    intros a I.
-    rewrite shift_of_abt_comm; auto.
-    eapply Forall_forall; eauto.
-  Qed.
-
-  Lemma identity_subst_of_abt :
+  Lemma identity_subst_to_abt_comm :
     forall n,
-      identity_subst n = List.map of_abt (A.identity_subst n).
+      List.map to_abt (identity_subst n) = A.identity_subst n.
   Proof.
     induction n; simpl; f_equal; auto.
-    rewrite IHn.
-    rewrite map_shift_of_abt_comm; auto.
-    apply A.ws_identity_subst.
+    now rewrite map_shift_to_abt_comm, IHn.
   Qed.
+End expr_basis.
 
-  Lemma wf_shift : forall e c d n, wf n e -> wf (d + n) (shift c d e).
-  Proof.
-    intros.
-    rewrite shift_to_of_abt.
-    rewrite wf_of_abt; auto.
-    apply A.wf_shift.
-    now rewrite <- wf_to_abt.
-  Qed.
-
-  Lemma wf_subst : forall e n rho, wf (length rho) e -> Forall (wf n) rho -> wf n (subst rho e).
-  Proof.
-    intros e n rho WF F.
-    rewrite subst_to_of_abt.
-    rewrite wf_of_abt.
-    - apply A.wf_subst.
-      + now rewrite map_length, <- wf_to_abt.
-      + rewrite Forall_map.
-        eapply Forall_impl; try eassumption.
-        intros e' WF'.
-        now rewrite <- wf_to_abt.
-    - apply A.ws_subst; auto.
-      rewrite Forall_map.
-      apply Forall_forall; auto.
-  Qed.
-
-  Lemma identity_subst_length : forall n, length (identity_subst n) = n.
-  Proof.
-    intros.
-    rewrite identity_subst_of_abt.
-    rewrite map_length.
-    apply A.identity_subst_length.
-  Qed.
-
-  Lemma wf_identity_subst: forall n : nat, Forall (wf n) (identity_subst n).
-  Proof.
-    intros.
-    rewrite identity_subst_of_abt.
-    rewrite Forall_map.
-    rewrite Forall_forall.
-    intros e I.
-    rewrite wf_of_abt.
-    - eapply Forall_forall; [apply A.wf_identity_subst|]; auto.
-    - eapply Forall_forall; [apply A.ws_identity_subst|]; eauto.
-  Qed.
-
-  Lemma wf_weaken : forall e n d, n <= d -> wf n e -> wf d e.
-  Proof.
-    intros e n d LE.
-    rewrite !wf_to_abt.
-    eauto using A.wf_weaken.
-  Qed.
-
-  Lemma shift_merge : forall e c d1 d2 , shift c d2 (shift c d1 e) = shift c (d2 + d1) e.
-  Proof.
-    intros e c d1 d2.
-    rewrite !shift_to_of_abt.
-    rewrite to_of_abt by auto.
-    now rewrite A.shift_merge.
-  Qed.
-
-  Lemma shift_nop_d :
-    forall e c,
-      shift c 0 e = e.
-  Proof.
-    intros e c.
-    rewrite shift_to_of_abt.
-    rewrite A.shift_nop_d.
-    now rewrite of_to_abt.
-  Qed.
-
-  Lemma subst_to_abt_comm : forall e rho, to_abt (subst rho e) = A.subst (map to_abt rho) (to_abt e).
-  Proof.
-    intros. rewrite subst_to_of_abt, to_of_abt; auto.
-    apply A.ws_subst; auto.
-    rewrite Forall_map.
-    apply Forall_forall.
-    auto.
-  Qed.
-
-  Lemma map_subst_to_abt_comm :
-    forall rho1 rho2,
-      map to_abt (map (subst rho2) rho1) =
-      map (A.subst (map to_abt rho2)) (map to_abt rho1).
-  Proof.
-    intros rho1 rho2.
-    rewrite !map_map.
-    apply map_ext.
-    intros e'.
-    auto using subst_to_abt_comm.
-  Qed.
-
-  Lemma subst_subst :
-    forall e rho1 rho2,
-      wf (List.length rho1) e ->
-      List.Forall (wf (List.length rho2)) rho1 ->
-      subst rho2 (subst rho1 e) =
-      subst (List.map (subst rho2) rho1) e.
-  Proof.
-    intros e rho1 rho2 WF F.
-    rewrite !subst_to_of_abt.
-    rewrite !to_of_abt.
-    - rewrite A.subst_subst.
-      + now rewrite map_subst_to_abt_comm.
-      + now rewrite map_length, <- wf_to_abt.
-      + rewrite map_length, Forall_map.
-        eapply Forall_impl; try eassumption.
-        intros e'.
-        now rewrite wf_to_abt.
-    - apply A.ws_subst; auto.
-      rewrite Forall_map.
-      apply Forall_forall; auto.
-  Qed.
-
-  Lemma subst_shift_singleton :
-    forall e e',
-      wf 0 e ->
-      subst [e'] (shift 0 1 e) = e.
-  Proof.
-    intros.
-    rewrite subst_to_of_abt, shift_to_of_abt.
-    simpl.
-    rewrite to_of_abt.
-    - rewrite A.subst_shift_singleton.
-      + now rewrite of_to_abt.
-      + now rewrite <- wf_to_abt.
-    - apply A.ws_shift; auto.
-  Qed.
-
-  Lemma subst_identity :
-    forall e n,
-      subst (identity_subst n) e = e.
-  Proof.
-    intros e n.
-    rewrite subst_to_of_abt, identity_subst_of_abt.
-    rewrite !map_map.
-    erewrite map_ext_in.
-    rewrite map_id.
-    rewrite A.subst_identity.
-    now rewrite of_to_abt.
-    intros e' I.
-    simpl.
-    rewrite to_of_abt; auto.
-    eapply Forall_forall.
-    apply A.ws_identity_subst.
-    eauto.
-  Qed.
+Module expr.
+  Include abt.abt_util expr_basis.
+  Notation var := expr_ast.var.
+  Notation abs := expr_ast.abs.
+  Notation app := expr_ast.app.
+  Notation tyabs := expr_ast.tyabs.
+  Notation tyapp := expr_ast.tyapp.
 End expr.
 
 Module has_type.
@@ -680,7 +331,7 @@ Module has_type.
       Forall (type.wf n) G ->
       type.wf n ty.
   Proof.
-    induction 1; cbn in *; intuition.
+    induction 1; cbn in *; intros F; intuition.
     - now eapply Forall_nth; eauto.
     - apply IHt.
       rewrite Forall_map.
